Tests.dfy
@@ -4,21 +4,30 @@ module Tests{
     import opened StaticAnalyzer
 
     method TestCase1(){
+        /*
+        v := 4 + 4;
+        v := v / 2;
+        */
         var stmt1 := Assign("v", Add(Const(4), Const(4)));
         var stmt2 := Assign("v", Div(Var("v"), Const(2)));
         var stmt3 := Seq(stmt1, stmt2);
         var env := map[];
+        var state := map[];
         
         AnalyzeProgramSound(stmt3, env);
-        assert AnalyzeStmt(stmt3, {}).0;
+        assert AnalyzeStmt(stmt3, state).0;
         match ExecStmt(stmt3, env)
         case Ok(env1) => assert env1["v"] == 4;
         case Err(e1) => assert false;
     }
 
     method TestCase2(){
+        /*
+        y := x + 1;
+        */
         var stmt := Assign("y", Add(Var("x"), Const(1)));
-        assert !AnalyzeStmt(stmt, {}).0;
+        var state := map[];
+        assert !AnalyzeStmt(stmt, state).0;
         var env := map[];
         
         match ExecStmt(stmt, env)
@@ -27,15 +36,23 @@ module Tests{
     }
 
     method TestCase3(){
+        /*
+        if(1){
+            x := 1;
+        } else{
+            x := 0;
+        }
+        */
         var cond_expr := Const(1);
         var stmt_then := Assign("x", Const(1));
         var stmt_else := Assign("x", Const(0));
         var stmt := If(cond_expr, stmt_then, stmt_else);
         var env := map[];
+        var state := map[];
 
         AnalyzeProgramSound(stmt, env);
 
-        assert AnalyzeStmt(stmt, {}).0;
+        assert AnalyzeStmt(stmt, state).0;
         
         match ExecStmt(stmt, env)
         case Ok(env1) => assert env1["x"] == 1;
@@ -43,14 +60,23 @@ module Tests{
     }
 
     method TestCase4(){
+        /*
+        if(1){
+            x := 1;
+        } else{
+            y := 0;
+        }
+        z := x;
+        */
         var cond_expr := Const(1);
         var stmt_then := Assign("x", Const(1));
         var stmt_else := Assign("y", Const(0));
         var if_stmt := If(cond_expr, stmt_then, stmt_else);
         var stmt := Seq(if_stmt, Assign("z", Var("x")));
         var env := map[];
+        var state := map[];
 
-        assert !AnalyzeStmt(stmt, {}).0;    
+        assert AnalyzeStmt(stmt, state).0;    
         
         match ExecStmt(stmt, env)
         case Ok(env1) => assert env1["x"] == 1;
@@ -58,10 +84,14 @@ module Tests{
     }
 
     method TestCase5(){
+        /*
+        z := 1 / 0;
+        */
         var stmt := Assign("z", Div(Const(1), Const(0)));
         var env := map[];
+        var state := map[];
 
-        assert !AnalyzeStmt(stmt, {}).0;
+        assert !AnalyzeStmt(stmt, state).0;
         
         match ExecStmt(stmt, env)
         case Ok(env1) => assert false;
@@ -69,10 +99,14 @@ module Tests{
     }
 
     method TestCase6(){
+        /*
+        z := 12 / (2 + 2);
+        */
         var stmt := Assign("z", Div(Const(12), Add(Const(2), Const(2))));
         var env := map[];
+        var state := map[];
 
-        assert !AnalyzeStmt(stmt, {}).0;
+        assert !AnalyzeStmt(stmt, state).0;
         
         match ExecStmt(stmt, env)
         case Ok(env1) => assert env1["z"] == 3;
@@ -80,15 +114,42 @@ module Tests{
     }
 
     method TestCase7(){
+        /*
+        if(1 + (-1)){
+            v := 30;
+        } else{
+            v := 4 * 4;
+            v := v - 2;
+        }
+        */
         var cond := Add(Const(1), Const(-1));
         var stmt1 := Assign("v", Mul(Const(4), Const(4)));
         var stmt2 := Assign("v", Sub(Var("v"), Const(2)));
         var stmt3 := If(cond, Assign("v", Const(30)), Seq(stmt1, stmt2));
+        var state := map[];
         
-        assert AnalyzeStmt(stmt3, {}).0;
+        assert AnalyzeStmt(stmt3, state).0;
         var env := map[];
         match ExecStmt(stmt3, env)
         case Ok(env1) => assert env1["v"] == 14;
+        case Err(e1) => assert false;
+    }
+
+    method TestCase8(){
+        /*
+        v := 4 + 4;
+        v := v % 2;
+        */
+        var stmt1 := Assign("v", Add(Const(4), Const(4)));
+        var stmt2 := Assign("v", Mod(Var("v"), Const(2)));
+        var stmt3 := Seq(stmt1, stmt2);
+        var env := map[];
+        var state := map[];
+        
+        AnalyzeProgramSound(stmt3, env);
+        assert AnalyzeStmt(stmt3, state).0;
+        match ExecStmt(stmt3, env)
+        case Ok(env1) => assert env1["v"] == 0;
         case Err(e1) => assert false;
     }
 }
